src/lib/poly/gemm/Kuiper.Poly.GEMM.TensorCore2D.KernelDesc.fst
@@ -251,24 +251,6 @@ fn setup
   ()
 }
 
-#push-options "--debug SMTFail --split_queries always"
-let bij_tile_stride_cells (et : Type0) {| sized et, hvc : has_vec_cpy et|} (#nthr : nat) (tid : natlt nthr)
-  (rows cols : nat) (#_: squash (chunk et  * nthr /?+ (rows * cols))) (#_: squash (chunk et /?+ cols))
-: (natlt (rows*cols/(chunk et * nthr)) =~ idx:natlt (rows*cols) {tid = idx/(chunk et) % nthr /\ chunk et /?+ idx /\ idx%cols < cols - chunk et + 1})
-=
-{
-  ff = admit(); //(fun (i : natlt (rows*cols/(chunk et * nthr))) ->
-    //assume (tid = (i * (chunk et * nthr) + tid * chunk et)/(chunk et) % nthr);
-    //assume (chunk et /?+ (i * (chunk et * nthr) + tid * chunk et));
-    //assume ((i * (chunk et * nthr) + tid * chunk et)%cols < cols - chunk et + 1);
-    //i * (chunk et * nthr) + tid * chunk et
-    // <: (idx:natlt (rows*cols) {tid = idx/(chunk et) % nthr /\ chunk et /?+ idx /\ idx%cols < cols - chunk et + 1}));
-  gg = (fun (i : natlt (rows*cols) {tid = i/(chunk et #_ #hvc) % nthr /\ (chunk et #_ #hvc) /?+ i /\ i%cols < cols - (chunk et #_ #hvc) + 1}) ->
-    i/(chunk et * nthr) <: natlt (rows*cols/(chunk et * nthr)));
-  ff_gg = ez;
-  gg_ff = ez;
-}
- 
 ghost
 fn single_even_barrier_p_to_q
   (#et : Type0) {| sized et, has_vec_cpy et |}
@@ -278,135 +260,20 @@ fn single_even_barrier_p_to_q
   (nthr : pos)
   (#_ : squash (chunk et /?+ cols))
   (#_ : squash (chunk et * nthr /?+ (rows * cols)))
-requires
-  forall+ (tid : natlt nthr).
-    (exists* (x : ematrix _ _ _). (from_array l sar) |-> Frac (1.0R /. nthr) x)
-ensures
-  forall+ (tid : natlt nthr).
-    live_tile_stride_cells (from_array l sar) nthr tid
+  requires
+    forall+ (tid : natlt nthr).
+      (exists* (x : ematrix _ _ _). (from_array l sar) |-> Frac (1.0R /. nthr) x)
+  ensures
+    forall+ (tid : natlt nthr).
+      live_strided_chunks (from_array l sar) nthr tid
 {
   gpu_matrix_gather_n_underspec (from_array l sar) nthr;
-  with em1. assert (from_array l sar) |-> em1;
-  gpu_matrix_explode _;
-  forevery_unfactor' (rows*cols) rows cols _;
-
-  Kuiper.Divides.lemma_divides_product_r (chunk et) cols rows;
-  assert pure (rows * cols / (chunk et) * (chunk et) == rows * cols);
-  forevery_factor (rows*cols) (rows*cols/chunk et) (chunk et) _;
-  with em'. assert
-    forall+ (i : natlt (rows*cols/chunk et)).
-      forall+ (k : natlt (chunk et)).
-        gpu_matrix_pts_to_cell (from_array l sar)
-          ((i * chunk et + k) / cols)
-          ((i * chunk et + k) % cols)
-          (macc em'
-            ((i * chunk et + k) / cols)
-            ((i * chunk et + k) % cols));
-
-  (*
-  open Pulse.Lib.WithPure;
-  ghost
-  fn aux_cell (i : natlt (rows*cols/chunk et)) (k : natlt (chunk et))
-  requires
-    gpu_matrix_pts_to_cell (from_array l sar)
-      ((i * chunk et + k) / cols) ((i * chunk et + k) % cols)
-      (macc em' ((i * chunk et + k) / cols) ((i * chunk et + k) % cols))
-  ensures
-      with_pure (i * chunk et % cols + k < cols)
-        (fun _ -> live_cell (from_array l sar) (i * chunk et / cols) (i * chunk et % cols + k))
-  {
-    assert pure (chunk et /?+ cols /\ k < chunk et); 
-    assert pure (i * chunk et < rows*cols-chunk et + 1);
-    assert pure (i * chunk et + k < (i+1) * chunk et);
-    // assert pure ((i * chunk et) % cols < cols - chunk et + 1);
-    // assert pure ((i * chunk et + k) % cols = i * chunk et % cols + k);
-    // assert pure (exists j. i * chunk et % cols = i * chunk et / cols + j * chunk et);
-    assume pure (((i * chunk et + k) / cols) = i * chunk et / cols);
-    assume pure (((i * chunk et + k) % cols) = i * chunk et % cols + k);
-    rewrite each ((i * chunk et + k) / cols) as (i * chunk et / cols);
-    rewrite each ((i * chunk et + k) % cols) as (i * chunk et % cols + k);
-    fold live_cell (from_array l sar) (i * chunk et / cols) (i * chunk et % cols +k);
-  };
-  forevery_map_2 _ _ aux_cell;
-  admit();
-
-  ghost
-  fn aux_chunk (i : natlt (rows*cols/chunk et))
-  requires
-    forall+ (k : natlt (chunk et)).
-      with_pure (i * chunk et % cols + k < cols)
-        (fun _ -> live_cell (from_array l sar) (i * chunk et / cols) (i * chunk et % cols + k))
-  ensures
-    with_pure (i * chunk et % cols < cols - chunk et + 1)
-      (fun _ -> live_chunk (from_array l sar) (i * chunk et / cols) (i * chunk et % cols))
-  {
-    admit(); 
-    fold live_chunk (from_array l sar) (i * chunk et / cols) (i * chunk et % cols);
-  };
-  admit();
-  *)
-
-  forevery_factor (rows*cols/chunk et) nthr (rows*cols/(chunk et * nthr)) _;
-  
-  with em. assert
-    forall+ (tid : natlt nthr).
-      forall+ (i : natlt (rows*cols/(chunk et * nthr))).
-        forall+ (k : natlt (chunk et)).
-          gpu_matrix_pts_to_cell (from_array l sar)
-                  (((tid * (rows * cols / (chunk et * nthr)) + i) * chunk et + k) / cols)
-                  (((tid * (rows * cols / (chunk et * nthr)) + i) * chunk et + k) % cols)
-                  (macc em
-                      (((tid * (rows * cols / (chunk et * nthr)) + i) * chunk et + k) / cols)
-                      (((tid * (rows * cols / (chunk et * nthr)) + i) * chunk et + k) % cols));
-  ghost
-  fn aux (tid : natlt nthr)
-  requires
-    forall+ (i : natlt (rows*cols/(chunk et * nthr))).
-      forall+ (k : natlt (chunk et)).
-        gpu_matrix_pts_to_cell (from_array l sar)
-          (((tid * (rows * cols / (chunk et * nthr)) + i) * chunk et + k) / cols)
-          (((tid * (rows * cols / (chunk et * nthr)) + i) * chunk et + k) % cols)
-          (macc em
-              (((tid * (rows * cols / (chunk et * nthr)) + i) * chunk et + k) / cols)
-              (((tid * (rows * cols / (chunk et * nthr)) + i) * chunk et + k) % cols))
-  ensures
-    live_tile_stride_cells (from_array l sar) nthr tid
-  {
-    forevery_iso #(natlt (rows*cols/(chunk et * nthr))) (bij_tile_stride_cells et tid rows cols) _;
-    admit();
-    ghost
-    fn aux2 (idx : natlt (rows*cols) {tid = idx/(chunk et) % nthr /\ chunk et /?+ idx /\ idx%cols < cols - chunk et + 1})
-    requires
-      forall+ (k : natlt (chunk et)).
-        gpu_matrix_pts_to_cell (from_array l sar)
-          (((tid * (rows * cols / (chunk et * nthr)) + idx) * chunk et + k) / cols)
-          (((tid * (rows * cols / (chunk et * nthr)) + idx) * chunk et + k) % cols)
-          (macc em
-              (((tid * (rows * cols / (chunk et * nthr)) + idx) * chunk et + k) / cols)
-              (((tid * (rows * cols / (chunk et * nthr)) + idx) * chunk et + k) % cols))
-    ensures
-      live_chunk (from_array l sar) (idx/cols) (idx%cols)
-    {
-      //ghost
-      //fn aux3 (k : natlt (chunk et))
-      //requires
-      //  gpu_matrix_pts_to_cell (from_array l sar)
-      //    (((tid * (rows * cols / (chunk et * nthr)) + i) * chunk et + k) / cols)
-      //    (((tid * (rows * cols / (chunk et * nthr)) + i) * chunk et + k) % cols)
-      //    (macc em
-      //        (((tid * (rows * cols / (chunk et * nthr)) + i) * chunk et + k) / cols)
-      //        (((tid * (rows * cols / (chunk et * nthr)) + i) * chunk et + k) % cols))
-      //ensures live_cell (from_array l sar) (((tid * (rows * cols / (chunk et * nthr)) + i) * chunk et) / cols) ()
-      admit();
-      fold live_chunk (from_array l sar) (idx/cols) (idx%cols);
-    };
-    forevery_map _ _ aux2;
-    admit();
-    ()
-  };
-
-  forevery_map _ _ aux;
-  ()
+  with em. assert (from_array l sar) |-> em;
+  split_matrix_into_strided_chunks (from_array l sar) nthr;
+  forevery_map
+    (fun tid -> own_strided_chunks (from_array l sar) em nthr tid)
+    (fun tid -> live_strided_chunks (from_array l sar) nthr tid)
+    fn tid { fold live_strided_chunks (from_array l sar) nthr tid; };
 }
 
 ghost
@@ -422,43 +289,20 @@ fn even_barrier_p_to_q
   (#_ : squash (chunk et /?+ bk))
   (#_ : squash (chunk et * nthr /?+ (bm * bk)))
   (#_ : squash (chunk et * nthr /?+ (bk * bn)))
-requires
-  forall+ (tid : natlt nthr).
-    (exists* (x : ematrix _ _ _). (from_array l1 sar1) |-> Frac (recip nthr) x) **
-    (exists* (x : ematrix _ _ _). (from_array l2 sar2) |-> Frac (recip nthr) x)
-ensures
-  forall+ (tid : natlt nthr).
-    live_tile_stride_cells (from_array l1 sar1) nthr tid **
-    live_tile_stride_cells (from_array l2 sar2) nthr tid
+  requires
+    forall+ (tid : natlt nthr).
+      (exists* (x : ematrix _ _ _). (from_array l1 sar1) |-> Frac (recip nthr) x) **
+      (exists* (x : ematrix _ _ _). (from_array l2 sar2) |-> Frac (recip nthr) x)
+  ensures
+    forall+ (tid : natlt nthr).
+      live_strided_chunks (from_array l1 sar1) nthr tid **
+      live_strided_chunks (from_array l2 sar2) nthr tid
 {
   forevery_unzip _ _;
   single_even_barrier_p_to_q l1 sar1 nthr;
   single_even_barrier_p_to_q l2 sar2 nthr;
   forevery_zip (fun (tid: natlt nthr) ->
-      live_tile_stride_cells (from_array l1 sar1) nthr tid) _;
-}
-
-let lemma_divides_prod_divisor (d1 d2 : pos) (a : nat)
-  : Lemma (requires (d1 * d2) /? a)
-          (ensures d1 /? a /\ d2 /? a)
-= admit()
-
-ghost
-fn gpu_matrix_implode_underspec
-  (#et:Type0)
-  (#rows #cols : nat)
-  (#l : mlayout rows cols)
-  (gm : gpu_matrix et l)
-  (#f : perm)
-  requires
-    pure (SZ.fits (mlayout_size l))
-  requires
-    forall+ r c.
-      exists* v. gpu_matrix_pts_to_cell gm #f r c v
-  ensures
-    exists* em. gpu_matrix_pts_to gm #f em
-{
-  admit();
+      live_strided_chunks (from_array l1 sar1) nthr tid) _;
 }
 
 ghost
@@ -470,51 +314,20 @@ fn single_odd_barrier_p_to_q
   (nthr : pos)
   (#_ : squash (chunk et /?+ cols))
   (#_ : squash (chunk et * nthr /?+ (rows * cols)))
-requires
-  forall+ (tid : natlt nthr). live_tile_stride_cells (from_array l sar) nthr tid
-ensures
-  forall+ (tid : natlt nthr).
-    (exists* (em : ematrix _ _ _). (from_array l sar) |-> Frac (recip nthr) em)
-{
-  ghost
-  fn aux (tid : natlt nthr)
+  (#_ : squash (SZ.fits (mlayout_size l)))
   requires
-    live_tile_stride_cells (from_array l sar) nthr tid
+    forall+ (tid : natlt nthr). live_strided_chunks (from_array l sar) nthr tid
   ensures
-    forall+ (idx : natlt (rows*cols) {tid = idx/(chunk et) % nthr /\ chunk et /?+ idx /\ idx%cols < cols - chunk et + 1}).
-      forall+ (k : natlt (chunk et)).
-        live_cell (from_array l sar) (idx/cols) (idx%cols + k)
-  {
-    unfold live_tile_stride_cells (from_array l sar);
-
-    forevery_iso_back (bij_tile_stride_cells et tid rows cols)
-      (fun i -> live_chunk (from_array l sar) ((i * (chunk et * nthr)) / cols) ((i * (chunk et * nthr)) % cols));
-    admit();
-  };
-  forevery_map _ _ aux;
-  admit();
-
-  forevery_unfactor' (rows*cols/chunk et) nthr (rows*cols/(chunk et * nthr)) _;
-  Kuiper.Divides.lemma_divides_exact (chunk et) (rows*cols);
-  lemma_divides_prod_divisor (chunk et) nthr (rows*cols);
-  forevery_unfactor' (rows*cols) (rows*cols/chunk et) (chunk et) _;
-
-  forevery_factor (rows*cols) rows cols _;
-  admit();
-  gpu_matrix_implode_underspec _;
-  with em1. assert (from_array l sar) |-> em1;
-  gpu_matrix_gather_n_underspec (from_array l sar) nthr;
-
-//  ((((i1 * cols + i2) / chunk /
-//                (rows * cols / (chunk * nthr)) *
-//                (rows * cols / (chunk * nthr)) +
-//                (i1 * cols + i2) /
-//                chunk %
-//                (rows * cols / (chunk * nthr))) *
-//
-//              chunk +
-//              (i1 * cols + i2) % chunk) /
-//            cols)
+    forall+ (tid : natlt nthr).
+      (exists* (em : ematrix _ _ _). (from_array l sar) |-> Frac (recip nthr) em)
+{
+  join_matrix_from_strided_chunks_underspec (from_array l sar) nthr;
+  with em. assert (from_array l sar) |-> em;
+  gpu_matrix_share_n (from_array l sar) nthr;
+  forevery_map
+    (fun (tid : natlt nthr) -> from_array l sar |-> Frac (recip nthr) em)
+    (fun (tid : natlt nthr) -> exists* (em : ematrix _ _ _). (from_array l sar) |-> Frac (recip nthr) em)
+    fn tid { (); };
 }
 
 ghost
@@ -530,10 +343,12 @@ fn odd_barrier_p_to_q
   (#_ : squash (chunk et /?+ bk))
   (#_ : squash (chunk et * nthr /?+ (bm * bk)))
   (#_ : squash (chunk et * nthr /?+ (bk * bn)))
+  (#_ : squash (SZ.fits (mlayout_size l1)))
+  (#_ : squash (SZ.fits (mlayout_size l2)))
 requires
   forall+ (tid : natlt nthr).
-    live_tile_stride_cells (from_array l1 sar1) nthr tid **
-    live_tile_stride_cells (from_array l2 sar2) nthr tid
+    live_strided_chunks (from_array l1 sar1) nthr tid **
+    live_strided_chunks (from_array l2 sar2) nthr tid
 ensures
   forall+ (tid : natlt nthr).
     (exists* (x : ematrix _ _ _). (from_array l1 sar1) |-> Frac (recip nthr) x) **
@@ -561,6 +376,8 @@ fn barrier_p_to_q_transform
   (#_ : squash (chunk et /?+ bk))
   (#_ : squash (chunk et * nthr /?+ (bm * bk)))
   (#_ : squash (chunk et * nthr /?+ (bk * bn)))
+  (#_ : squash (SZ.fits (mlayout_size l1)))
+  (#_ : squash (SZ.fits (mlayout_size l2)))
   (it : nat)
 requires
   forall+ (tid : natlt nthr). barrier_p (from_array l1 sar1) (from_array l2 sar2) nthr it tid
@@ -590,13 +407,13 @@ ensures
     ghost
     fn evaux2 (tid : natlt nthr)
     requires
-      live_tile_stride_cells (from_array l1 sar1) nthr tid **
-      live_tile_stride_cells (from_array l2 sar2) nthr tid
+      live_strided_chunks (from_array l1 sar1) nthr tid **
+      live_strided_chunks (from_array l2 sar2) nthr tid
     ensures
       barrier_q (from_array l1 sar1) (from_array l2 sar2) nthr it tid
     {
-      rewrite live_tile_stride_cells (from_array l1 sar1) nthr tid **
-              live_tile_stride_cells (from_array l2 sar2) nthr tid
+      rewrite live_strided_chunks (from_array l1 sar1) nthr tid **
+              live_strided_chunks (from_array l2 sar2) nthr tid
            as barrier_q (from_array l1 sar1) (from_array l2 sar2) nthr it tid;
     };
     forevery_map _ _ evaux2;
@@ -607,12 +424,12 @@ ensures
       requires
         barrier_p (from_array l1 sar1) (from_array l2 sar2) nthr it tid
       ensures
-        live_tile_stride_cells (from_array l1 sar1) nthr tid **
-        live_tile_stride_cells (from_array l2 sar2) nthr tid
+        live_strided_chunks (from_array l1 sar1) nthr tid **
+        live_strided_chunks (from_array l2 sar2) nthr tid
     {
       rewrite barrier_p (from_array l1 sar1) (from_array l2 sar2) nthr it tid
-           as live_tile_stride_cells (from_array l1 sar1) nthr tid **
-              live_tile_stride_cells (from_array l2 sar2) nthr tid;
+           as live_strided_chunks (from_array l1 sar1) nthr tid **
+              live_strided_chunks (from_array l2 sar2) nthr tid;
     };
 
     forevery_map _ _ oddaux;
@@ -637,15 +454,15 @@ ensures
           (exists* (x : ematrix _ _ _). (from_array l1 sar1) |-> Frac (recip nthr) x) **
           (exists* (x : ematrix _ _ _). (from_array l2 sar2) |-> Frac (recip nthr) x)
         else
-          live_tile_stride_cells (from_array l1 sar1) nthr tid **
-          live_tile_stride_cells (from_array l2 sar2) nthr tid);
+          live_strided_chunks (from_array l1 sar1) nthr tid **
+          live_strided_chunks (from_array l2 sar2) nthr tid);
       rewrite
         (if even (it+1) then
           (exists* (x : ematrix _ _ _). (from_array l1 sar1) |-> Frac (recip nthr) x) **
           (exists* (x : ematrix _ _ _). (from_array l2 sar2) |-> Frac (recip nthr) x)
         else
-          live_tile_stride_cells (from_array l1 sar1) nthr tid **
-          live_tile_stride_cells (from_array l2 sar2) nthr tid)
+          live_strided_chunks (from_array l1 sar1) nthr tid **
+          live_strided_chunks (from_array l2 sar2) nthr tid)
       as
         barrier_q (from_array l1 sar1) (from_array l2 sar2) nthr it tid;
     };
@@ -727,12 +544,6 @@ fn block_setup
   forevery_map #(natlt nthr)
     (fun _tid -> gpu_pts_to_slice (fst (snd sh)) #(recip nthr) 0 (bk*bn) s2)
     _ (aux (fst (snd sh)) s2);
-  forevery_map
-    (fun _tid -> gpu_pts_to_slice (fst sh) #(1.0R /. nthr) 0 (bm*bk) s1) _
-    (aux (fst sh) s1);
-  forevery_map
-    (fun _tid -> gpu_pts_to_slice (fst (snd sh)) #(1.0R /. nthr) 0 (bk*bn) s2) _
-    (aux (fst (snd sh)) s2);
 
   (* create barrier token *)
   B.mk_barrier nthr _ _
