src/lib/kuiper/Kuiper.ForEvery.fsti
@@ -911,3 +911,50 @@ fn forevery_unflatten4'
     forall+ (xyzw : a & b & c & d). f xyzw
   ensures
     forall+ (x:a) (y:b) (z:c) (w:d). f (x, y, z, w)
+
+
+
+ghost
+fn forevery_split_or_2
+  (#a:Type0)
+  (r s : a -> prop)
+  (p : a -> slprop)
+  requires
+    pure (~ (exists (x:a). r x /\ s x))
+  requires
+    forall+ (x:a { r x \/ s x }). p x
+  ensures
+    (forall+ (x:a { r x }). p x) **
+    (forall+ (x:a { s x }). p x)
+
+ghost
+fn forevery_split_or_n
+  (#a:Type0)
+  (n : nat)
+  (r : natlt n -> a -> prop)
+  (p : a -> slprop)
+  requires
+    pure (forall (i1 i2 : natlt n) x.
+      r i1 x /\ r i2 x ==> i1 == i2)
+  requires
+    forall+ (x:a {exists i. r i x}). p x
+  ensures
+    forall+ (i : natlt n).
+      forall+ (x:a { r i x }).
+        p x
+
+ghost
+fn forevery_join_or_n
+  (#a:Type0)
+  (n : nat)
+  (r : natlt n -> a -> prop)
+  (p : a -> slprop)
+  requires
+    pure (forall (i1 i2 : natlt n) x.
+      r i1 x /\ r i2 x ==> i1 == i2)
+  requires
+    forall+ (i : natlt n).
+      forall+ (x:a { r i x }).
+        p x
+  ensures
+    forall+ (x:a {exists i. r i x}). p x
